wip proving the request-down case of serializability

src/RqDownRed.v
@@ -37,7 +37,7 @@ Section RqDownReduction.
 
     Lemma rqDown_olast_inside_tree:
       forall inits ins hst outs eouts,
-        DisjList inits rqDowns ->
+        DisjList rqDowns inits ->
         Atomic msg_dec inits ins hst outs eouts ->
         forall st1 st2 loidx,
           Reachable (steps step_m) sys st1 ->
@@ -51,7 +51,7 @@ Section RqDownReduction.
 
     Lemma rqDown_olast_outside_tree:
       forall inits ins hst outs eouts,
-        DisjList inits rqDowns ->
+        DisjList rqDowns inits ->
         Atomic msg_dec inits ins hst outs eouts ->
         forall st1 st2 loidx,
           Reachable (steps step_m) sys st1 ->
@@ -59,14 +59,130 @@ Section RqDownReduction.
           steps step_m sys st1 hst st2 ->
           lastOIdxOf hst = Some loidx ->
           ~ In loidx (subtreeIndsOf dtr oidxTo) ->
-          exists rqUps phst nhst,
+          exists phst rqUps ninits nins nhst nouts,
             hst = nhst ++ phst /\
-            RqUpHistory dtr phst rqUps /\
+            (phst = nil \/ RqUpHistory dtr phst rqUps) /\
             SubList (oindsOf phst) (subtreeIndsOf dtr oidxTo) /\
+            SubList ninits ins /\
+            Atomic msg_dec ninits nins nhst nouts eouts /\
             DisjList (oindsOf nhst) (subtreeIndsOf dtr oidxTo).
     Proof.
     Admitted.
 
+    Definition RqDownP (st: MState oifc) :=
+      Forall (InMPI st.(bst_msgs)) rqDowns.
+
+    Lemma rqDown_lpush_rpush_unit_reducible:
+      forall rinits rins rhst routs reouts
+             linits lins lhst louts leouts,
+        Atomic msg_dec rinits rins rhst routs reouts ->
+        DisjList (oindsOf rhst) (subtreeIndsOf dtr oidxTo) ->
+        Atomic msg_dec linits lins lhst louts leouts ->
+        SubList (oindsOf lhst) (subtreeIndsOf dtr oidxTo) ->
+        DisjList reouts linits ->
+        Reducible sys (lhst ++ rhst) (rhst ++ lhst).
+    Proof.
+      intros.
+      eapply rqrs_reducible; try eassumption.
+      eapply DisjList_comm, DisjList_SubList; [eassumption|].
+      apply DisjList_comm; assumption.
+    Qed.
+    
+    Lemma rqDown_lpush_unit_reducible:
+      forall pinits pins phst pouts peouts
+             inits ins hst outs eouts loidx,
+        PInitializing sys RqDownP phst ->
+        Atomic msg_dec pinits pins phst pouts peouts ->
+        SubList rqDowns peouts ->
+        Atomic msg_dec inits ins hst outs eouts ->
+        lastOIdxOf hst = Some loidx ->
+        In loidx (subtreeIndsOf dtr oidxTo) ->
+        DisjList peouts inits ->
+        Reducible sys (hst ++ phst) (phst ++ hst).
+    Proof.
+      intros; red; intros.
+      eapply steps_split in H6; [|reflexivity].
+      destruct H6 as [sti [? ?]].
+      eapply rqDown_lpush_rpush_unit_reducible; try eassumption.
+      - eapply rqDown_oinds; try eassumption.
+      - eapply rqDown_olast_inside_tree.
+        + eapply DisjList_SubList; [|eassumption].
+          eassumption.
+        + eassumption.
+        + eapply reachable_steps; [eassumption|].
+          eassumption.
+        + eapply H; eassumption.
+        + eassumption.
+        + eassumption.
+        + eassumption.
+      - eapply steps_append; eauto.
+    Qed.
+
+    Lemma rqDown_rpush_unit_reducible:
+      forall inits ins hst outs eouts loidx ridx routs,
+        Atomic msg_dec inits ins hst outs eouts ->
+        lastOIdxOf hst = Some loidx ->
+        ~ In loidx (subtreeIndsOf dtr oidxTo) ->
+        DisjList rqDowns inits ->
+        ReducibleP sys RqDownP (RlblInt oidxTo ridx rqDowns routs :: hst)
+                   (hst ++ [RlblInt oidxTo ridx rqDowns routs]).
+    Proof.
+      intros; red; intros.
+      inv_steps.
+      pose proof (rqDown_olast_outside_tree H2 H Hr Hp H7 H0 H1).
+      destruct H3 as [rhst [rqUps ?]].
+      destruct H3 as [ninits [nins [nhst [nouts ?]]]]; dest; subst.
+      eapply steps_split in H7; [|reflexivity].
+      destruct H7 as [sti [? ?]].
+
+      rewrite <-app_assoc.
+      eapply reducible_app_1; try assumption.
+      - instantiate (1:= RlblInt oidxTo ridx rqDowns routs :: rhst).
+        red; intros.
+        destruct H4; dest; subst; simpl in *.
+        + inv_steps.
+          apply steps_singleton; assumption.
+        + eapply rqUpHistory_lpush_lbl; try eassumption.
+          (* [RqUp]s and [RqDown]s are certainly disjoint. *)
+          admit.
+      - change (nhst ++ RlblInt oidxTo ridx rqDowns routs :: rhst)
+          with (nhst ++ [RlblInt oidxTo ridx rqDowns routs] ++ rhst).
+        rewrite app_assoc.
+        eapply reducible_app_2; try assumption.
+        + instantiate (1:= RlblInt oidxTo ridx rqDowns routs :: nhst).
+          change (RlblInt oidxTo ridx rqDowns routs :: nhst)
+            with ([RlblInt oidxTo ridx rqDowns routs] ++ nhst).
+          eapply rqDown_lpush_rpush_unit_reducible; try eassumption.
+          * constructor.
+          * simpl.
+            (* [In oidxTo (subtreeIndsOf dtr oidxTo)] when [oidxTo] is valid. *)
+            admit.
+          * (* For an [Atomic] history, 
+             * if [DisjList rqDowns inits] then [DisjList eouts rqDowns] *)
+            admit.
+        + simpl; econstructor; [|eassumption].
+          eapply steps_append; eassumption.
+    Admitted.      
+
+    Lemma rqDown_LRPushable_unit_reducible:
+      forall rinits rins rhst routs reouts rloidx
+             linits lins lhst louts leouts lloidx,
+        Atomic msg_dec rinits rins rhst routs reouts ->
+        DisjList rqDowns rinits ->
+        lastOIdxOf rhst = Some rloidx ->
+        ~ In rloidx (subtreeIndsOf dtr oidxTo) ->
+        Atomic msg_dec linits lins lhst louts leouts ->
+        DisjList rqDowns linits ->
+        lastOIdxOf lhst = Some lloidx ->
+        In lloidx (subtreeIndsOf dtr oidxTo) ->
+        ReducibleP sys RqDownP (lhst ++ rhst) (rhst ++ lhst).
+    Proof.
+      intros; red; intros.
+      eapply steps_split in H7; [|reflexivity].
+      destruct H7 as [sti [? ?]].
+      (* pose proof (rqDown_olast_outside_tree H2 H Hr Hp H7 H0 H1). *)
+    Admitted.
+    
   End OnRqDown.
 
 End RqDownReduction.
